ResolveKinds proofs

src/HiFirrtl.v
@@ -91,7 +91,7 @@ Section HiFirrtl.
   Inductive hfmodule : Type :=
   | FInmod : var -> seq hfport -> seq hfstmt -> hfmodule
   | FExmod : var -> seq hfport -> seq hfstmt -> hfmodule
-(* DNJ: External modules do not contain statements but only an interface.
+(* DNJ: External modules do not contain statements but only an interface. 
 They may contain the following special statements:
 one “defname = ...” (to set the Verilog name)
 zero, one, or multiple “parameter <variable> = <constant> (to pass parameters to the Verilog design that implements this module)
@@ -167,7 +167,7 @@ Module Type CmpntEnv (V : SsrOrder) <: SsrFMap.
 
   (* Return the env with a variable v, where the snd element of type is given *)
   Parameter add_snd : SE.t -> fcomponent -> env -> env.
-  Parameter Add_snd : SE.t -> fcomponent -> env -> env -> Prop.
+  Parameter Add_snd : SE.t -> fcomponent -> env -> env -> Prop. 
 
 End CmpntEnv.
 
@@ -218,7 +218,7 @@ Module MakeCmpntEnv (V : SsrOrder) (VM : SsrFMap with Module SE := V) <:
   Definition add_fst (v : V.t) (c : cmpnttyp) (e : env) : env :=
     let (f, s) := vtyp v e in add v (c, s) e.
   Definition add_snd (v : V.t) (fc : fcomponent) (e : env) : env :=
-    let (f, s) := vtyp v e in add v (f, fc) e.
+    let (f, s) := vtyp v e in add v (f, fc) e. 
   Definition Add_fst x c e e' := forall y, fst (vtyp y e') = fst (vtyp y (add_fst x c e)).
   Lemma Add_add_fst {v c e} : Add_fst v c e (add_fst v c e).
   Proof. done. Qed.
@@ -240,11 +240,11 @@ Section Rhs_expr.
   | R_default
   .
 
-
+  
   (** eq dec *)
   Axiom rhs_expr_eq_dec : forall {x y : rhs_expr}, {x = y} + {x <> y}.
   Parameter rhs_expr_eqn : forall (x y : rhs_expr), bool.
-  Axiom rhs_expr_eqP : Equality.axiom rhs_expr_eqn.
+  Axiom rhs_expr_eqP : Equality.axiom rhs_expr_eqn. 
   Canonical rhs_expr_eqMixin := EqMixin rhs_expr_eqP.
   Canonical rhs_expr_eqType := Eval hnf in EqType rhs_expr rhs_expr_eqMixin.
 
@@ -315,13 +315,13 @@ End StructStore.
 Module StructType (V:SsrOrder)<: HasDefaultTyp.
   Definition t : Type := rhs_expr V.T.
   Definition default : t := R_default V.T.
-
+  
 End StructType.
 
 Module MakeStructStore (V : SsrOrder) (CE : CmpntEnv V with Module SE := V) <:
   StructStore V CE.
   Module StructTypeV := StructType V.
-  Include MakeTStoreMap V StructTypeV.
+  Include MakeTStoreMap V StructTypeV. 
   Module Lemmas := FMapLemmas CE.
   Definition map2 (f : option (rhs_expr V.T) -> option (rhs_expr V.T) -> option (rhs_expr V.T)) (s1 s2 : t) : t :=
     M.map2 f s1 s2.
@@ -400,12 +400,12 @@ Module MakeHiFirrtl
   (** eq dec *)
   Axiom forient_eq_dec : forall {x y : forient}, {x = y} + {x <> y}.
   Parameter forient_eqn : forall (x y : forient), bool.
-  Axiom forient_eqP : Equality.axiom forient_eqn.
+  Axiom forient_eqP : Equality.axiom forient_eqn. 
   Canonical forient_eqMixin := EqMixin forient_eqP.
   Canonical forient_eqType := Eval hnf in EqType forient forient_eqMixin.
 
   Definition orient_of_comp c :=
-    match c with
+    match c with 
     | In_port | Instanceof | Memory | Node => Source
     (* DNJ: Not sure whether a memory should be a source. It is written like that
     in the specificiation, but actually the data type of a memory port is a bundle
@@ -467,9 +467,9 @@ Module MakeHiFirrtl
   (* ground type equivalence *)
   Definition fgtyp_equiv t1 t2 :=
     match t1, t2 with
-    | Fuint _, Fuint _
-    | Fsint _, Fsint _
-    | Fclock, Fclock
+    | Fuint _, Fuint _ 
+    | Fsint _, Fsint _ 
+    | Fclock, Fclock 
     | Freset, Freset
     (* | Freset, Fuint 1 *)
     | Fasyncreset, Fasyncreset => true
@@ -533,7 +533,7 @@ Module MakeHiFirrtl
   Fixpoint ftype_weak_equiv t1 t2 :=
     match t1, t2 with
     | Gtyp gt1, Gtyp gt2 => fgtyp_equiv gt1 gt2
-    | Atyp t1 n1, Atyp t2 n2 => ftype_equiv t1 t2
+    | Atyp t1 n1, Atyp t2 n2 => ftype_equiv t1 t2 
     | Btyp bt1, Btyp bt2 => fbtyp_weak_equiv bt1 bt2
     | _, _ => false
     end.
@@ -545,7 +545,7 @@ Module MakeHiFirrtl
   Definition unknown_typ := @Unknown_typ V.T.
 
 
-
+  
   Fixpoint eref_has_v (v:var) r :=
     match r with
     | Eid v1 => v1 == v
@@ -564,7 +564,7 @@ Module MakeHiFirrtl
     | Evalidif c e => fexpr_has_v v c || fexpr_has_v v e
     | Eref r => eref_has_v v r
     end.
-
+  
   (********************************************************************************)
 
   (** Pass Resolvekinds *)
@@ -572,19 +572,20 @@ Module MakeHiFirrtl
   (* Resolve component kind from statement, init with unknown type *)
   Inductive resolveKinds_stmt : hfstmt -> cenv -> cenv -> Prop :=
   | Resolve_wire v t (ce : cenv) (ce' : cenv) :
-      CELemmas.P.Add v (unknown_typ, Wire) ce ce' ->
+      CE.find v ce' = Some (unknown_typ, Wire) ->
       resolveKinds_stmt (swire v t) ce ce'
   | Resolve_reg v r ce ce' :
-      CELemmas.P.Add v (unknown_typ, Register) ce ce' ->
+      CE.find v ce' = Some (unknown_typ, Register) ->
       resolveKinds_stmt (sreg v r) ce ce'
   | Resolve_inst v1 v2 ce ce' :
-      CELemmas.P.Add v1 (unknown_typ, Instanceof) ce ce' ->
+  (*~~ (v1 == v2) ->*)
+      CE.find v1 ce' = Some (unknown_typ, Instanceof) ->
       resolveKinds_stmt (sinst v1 v2) ce ce'
   | Resolve_node v e ce ce' :
-      CELemmas.P.Add v (unknown_typ, Node) ce ce' ->
+      CE.find v ce' = Some (unknown_typ, Node) ->
       resolveKinds_stmt (snode v e) ce ce'
   | Resolve_mem v m ce ce' :
-      CELemmas.P.Add v (unknown_typ, Memory) ce ce' ->
+      CE.find v ce' = Some (unknown_typ, Memory) ->
       resolveKinds_stmt (smem v m) ce ce'
   | Resolve_invalid v ce :
       resolveKinds_stmt (sinvalid v) ce ce
@@ -612,10 +613,10 @@ Module MakeHiFirrtl
 
   Inductive resolveKinds_port : hfport -> CE.env -> CE.env -> Prop :=
   | Resolve_input v t ce ce' :
-      CELemmas.P.Add v (unknown_typ, In_port) ce ce' ->
+      CE.find v ce' = Some (unknown_typ, In_port) ->
       resolveKinds_port (Finput v t) ce ce'
   | Resolve_output v t ce ce' :
-      CELemmas.P.Add v (unknown_typ, Out_port) ce ce' ->
+      CE.find v ce' = Some (unknown_typ, Out_port) ->
       resolveKinds_port (Foutput v t) ce ce'
   .
 
@@ -628,12 +629,12 @@ Module MakeHiFirrtl
       resolveKinds_ports (p::ps) ce ce''.
 
   Inductive resolveKinds_module : hfmodule -> CE.env -> CE.env -> Prop :=
-  | Resolves_inmod vm ps ss ce ce' :
-      CELemmas.P.Add vm (unknown_typ, Fmodule) ce ce' ->
-      resolveKinds_module (hfinmod vm ps ss) ce ce
+  | Resolves_inmod vm ps ss ce ce' : 
+      CE.find vm ce' = Some (unknown_typ, Fmodule) ->
+      resolveKinds_module (hfinmod vm ps ss) ce ce'
   | Resolves_exmod vm ps ss ce ce' :
-      CELemmas.P.Add vm (unknown_typ, Fmodule) ce ce' ->
-      resolveKinds_module (hfexmod vm ps ss) ce ce
+      CE.find vm ce' = Some (unknown_typ, Fmodule) ->
+      resolveKinds_module (hfexmod vm ps ss) ce ce'
   .
 
   Inductive resolveKinds_modules : seq hfmodule -> CE.env -> CE.env -> Prop :=
@@ -691,26 +692,23 @@ Module MakeHiFirrtl
     resolveKinds_stmt (Snode v e) ce0 (resolveKinds_stmt_fun (Snode v e) ce0).
 Proof.
   intros. apply Resolve_node.
-  rewrite /resolveKinds_stmt_fun.
-  done.
-Qed.
+  rewrite /resolveKinds_stmt_fun /CE.add_fst (CELemmas.add_eq_o _ _ (eq_refl v)) //.
+  Qed.
 
 Lemma resolveKinds_sreg_sem_conform :
   forall v e ce0 ,
   resolveKinds_stmt (Sreg v e) ce0 (resolveKinds_stmt_fun (Sreg v e) ce0).
 Proof.
   intros. apply Resolve_reg.
-  rewrite /resolveKinds_stmt_fun.
-  done.
-Qed.
+  rewrite /resolveKinds_stmt_fun /CE.add_fst (CELemmas.add_eq_o _ _ (eq_refl v)) //.
+  Qed.
 
 Lemma resolveKinds_smem_sem_conform :
   forall v e ce0 ,
   resolveKinds_stmt (Smem v e) ce0 (resolveKinds_stmt_fun (Smem v e) ce0).
 Proof.
   intros. apply Resolve_mem.
-  rewrite /resolveKinds_stmt_fun.
-  done.
+  rewrite /resolveKinds_stmt_fun /CE.add_fst (CELemmas.add_eq_o _ _ (eq_refl v)) //.
 Qed.
 
 Lemma resolveKinds_sinvalid_sem_conform :
@@ -761,7 +759,7 @@ Lemma resolveKinds_swire_sem_conform :
 Proof.
   intros. apply Resolve_wire.
   rewrite /resolveKinds_stmt_fun.
-  done.
+  rewrite (CELemmas.add_eq_o _ _ (eq_refl v)) //.
 Qed.
   
 Lemma resolveKinds_sinst_sem_conform :
@@ -769,8 +767,7 @@ Lemma resolveKinds_sinst_sem_conform :
   resolveKinds_stmt (Sinst v1 v2) ce0 (resolveKinds_stmt_fun (Sinst v1 v2) ce0).
 Proof.
   intros. apply Resolve_inst.
-  rewrite /resolveKinds_stmt_fun.
-  done.
+  rewrite /resolveKinds_stmt_fun /CE.add_fst (CELemmas.add_eq_o _ _ (eq_refl v1)) //.
 Qed.
 
 Lemma resolveKinds_stmts_sem_conform : 
@@ -802,6 +799,7 @@ Lemma resolveKinds_inport_sem_conform :
   Proof.
     intros.
     apply Resolve_input; try done.
+    rewrite /resolveKinds_port_fun /CE.add_fst (CELemmas.add_eq_o _ _ (eq_refl v)) //.
     Qed.
 
 Lemma resolveKinds_outport_sem_conform :
@@ -810,6 +808,7 @@ Lemma resolveKinds_outport_sem_conform :
   Proof.
     intros.
     apply Resolve_output; try done.
+    rewrite /resolveKinds_port_fun /CE.add_fst (CELemmas.add_eq_o _ _ (eq_refl v)) //.
     Qed.
 
 Lemma resolveKinds_ports_sem_conform : 
@@ -831,12 +830,34 @@ forall vm ps ss ce,
   resolveKinds_module (FInmod vm ps ss) ce (resolveKinds_module_fun (FInmod vm ps ss) ce).
 Proof.
   intros.
+  apply Resolves_inmod.
   rewrite /resolveKinds_module_fun.
-  (*apply Resolves_inmod.*)
+  rewrite /CE.add_fst (CELemmas.add_eq_o _ _ (eq_refl vm)) //.
+Qed.
 
-Admitted.
+Lemma resolveKinds_exmod_sem_conform :
+forall vm ps ss ce,
+  resolveKinds_module (FExmod vm ps ss) ce (resolveKinds_module_fun (FExmod vm ps ss) ce).
+Proof.
+  intros.
+  apply Resolves_exmod.
+  rewrite /resolveKinds_module_fun.
+  rewrite /CE.add_fst (CELemmas.add_eq_o _ _ (eq_refl vm)) //.
+Qed.
 
-(* mods *)
+Lemma resolveKinds_mods_sem_conform :
+forall ms ce0 ,
+  resolveKinds_modules ms ce0 (resolveKinds_modules_fun ms ce0).
+Proof.
+    elim. intros. apply Resolve_modules_nil.
+    intros.
+    apply Resolve_modules_cons with (resolveKinds_module_fun a ce0).
+    elim a; intros;try done.
+    - apply resolveKinds_inmod_sem_conform.
+    - apply resolveKinds_exmod_sem_conform.
+    rewrite /=.
+    apply (H (resolveKinds_module_fun a ce0)).
+    Qed.
 
   (** decide the type and width of hifirrtl expressions *)
 
@@ -876,7 +897,7 @@ Admitted.
                        match t with
                        | Btyp fs => let fix aux fx := (
                                           match fx with
-                                          | Fflips v' f t fxs =>
+                                          | Fflips v' f t fxs => 
                                             if (v2var v == v') then t
                                             else aux fxs
                                           | Fnil => def_ftype
@@ -1067,7 +1088,7 @@ Admitted.
                                 end
     | Eprim_binop Band e1 e2
     | Eprim_binop Bor e1 e2
-    | Eprim_binop Bxor e1 e2 => let t1 := type_of_hfexpr e1 ce in
+    | Eprim_binop Bxor e1 e2 => let t1 := type_of_hfexpr e1 ce in 
                                 let t2 := type_of_hfexpr e2 ce in
                                 match t1, t2 with
                                 | Gtyp (Fuint w1), Gtyp (Fuint w2) => Gtyp (Fuint (maxn w1 w2))
@@ -1076,7 +1097,7 @@ Admitted.
                                 end
     | Emux c e1 e2 => let t1 := type_of_hfexpr e1 ce in
                       let t2 := type_of_hfexpr e2 ce in
-                      mux_types t1 t2
+                      mux_types t1 t2 
     | Evalidif c e1 => type_of_hfexpr e1 ce
     end.
 
@@ -1085,14 +1106,14 @@ Admitted.
 
 
    Parameter new_comp_name : var -> Prop.
-
+   
    Parameter new_v_cefind_none:
      forall v,
      new_comp_name v ->
      forall ce: cenv, CE.find v ce = None.
-
+  
   (** Pass InferType *)
-  (* infer type according to a statement *)
+  (* infer type according to a statement *) 
   Inductive inferType_stmt : hfstmt -> cenv -> cenv -> Prop :=
   | Infertype_wire v t ce ce' :
       new_comp_name v ->
@@ -1161,19 +1182,17 @@ Admitted.
 
   (*Inductive inferType_stmts : seq hfstmt -> cenv -> cenv -> Prop :=
   | Infertype_stmts_know ss ce ce' :
-      (exists v,
+      (exists v, 
                  ~~ find_unknown v ce') ->
       inferType_stmts (ss) ce ce'.*)
-
+  
   (* infer type according to ports declaration *)
   Inductive inferType_port : hfport -> cenv -> cenv -> Prop :=
   | Infertype_inport v t ce ce' :
-      CE.find v ce = None ->
-      ce' = CE.add v (aggr_typ t, In_port) ce ->
+      CE.find v ce' = Some (aggr_typ t, In_port) ->
       inferType_port (Finput v t) ce ce'
   | Infertype_outport v t ce ce' :
-      CE.find v ce = None ->
-      ce' = CE.add v (aggr_typ t, Out_port) ce ->
+      CE.find v ce' = Some (aggr_typ t, Out_port) ->
       inferType_port (Foutput v t) ce ce'.
 
   Inductive inferType_ports : seq hfport -> cenv -> cenv -> Prop :=
@@ -1249,7 +1268,7 @@ Admitted.
      forall v t e ce ce', new_comp_name v ->
                         ce' = CE.add v t ce ->
                         type_of_hfexpr e ce = type_of_hfexpr e ce'.
-
+                      
   Definition inferType_port_fun p ce :=
     match p with
     | Finput v t => CE.add v (aggr_typ t, In_port) ce
@@ -1362,7 +1381,7 @@ Admitted.
     intros. apply Infertype_node; try done.
     rewrite /inferType_stmt_fun (CELemmas.add_eq_o _ _ (eq_refl v)) //.
   Qed.
-
+  
   Lemma inferType_sreg_sem_conform :
     forall v r ce0 ,
       new_comp_name v ->
@@ -1397,7 +1416,7 @@ Admitted.
     rewrite /inferType_stmt_fun.
     rewrite (CELemmas.add_eq_o _ _ (eq_refl v)) //.
   Qed.
-
+    
   Lemma inferType_sinst_sem_conform :
     forall v1 v2  ce0 ,
       new_comp_name v1 ->
@@ -1415,7 +1434,7 @@ Admitted.
       type_of_cmpnttyp t = type_of_hfexpr e ce0 ->
       inferType_stmt (Sfcnct v1 e) ce0 (inferType_stmt_fun (Sfcnct v1 e) ce0).
   Proof.
-    intros.
+    intros. 
     rewrite /inferType_stmt_fun.
     apply Infertype_sfcnct with t (type_of_cmpnttyp t) c.
     split.
@@ -1456,7 +1475,7 @@ Admitted.
   Proof.
     intros. apply Infertype_sstop.
   Qed.
-
+    
   Lemma inferType_sskip_sem_conform :
   forall ce0 ,
       inferType_stmt sskip ce0 (inferType_stmt_fun sskip ce0).
@@ -1511,59 +1530,51 @@ Admitted.
 
   Lemma inferType_inport_sem_conform :
   forall v t ce0 ,
-      CE.find v ce0 = None ->
       inferType_port (Finput v t) ce0 (inferType_port_fun (Finput v t) ce0).
   Proof.
     intros.
-    apply Infertype_inport; try done.
-    Qed.
+    apply Infertype_inport.
+    rewrite (CELemmas.add_eq_o _ _ (eq_refl v)) //.
+  Qed.
 
   Lemma inferType_outport_sem_conform :
   forall v t ce0 ,
-      CE.find v ce0 = None ->
       inferType_port (Foutput v t) ce0 (inferType_port_fun (Foutput v t) ce0).
   Proof.
     intros.
-    apply Infertype_outport; try done.
-    Qed.
+    apply Infertype_outport.
+    rewrite (CELemmas.add_eq_o _ _ (eq_refl v)) //.
+  Qed.
 
   Lemma inferType_ports_sem_conform :
   forall ss ce0,
-    (forall v t, In (Finput v t) ss -> CE.find v ce0 = None) ->
-    (forall v t, In (Foutput v t) ss -> CE.find v ce0 = None) ->
     inferType_ports ss ce0 (inferType_ports_fun ss ce0).
   Proof.
     elim. intros. apply infertype_ports_nil.
     intros.
     apply infertype_ports_con with (inferType_port_fun a ce0).
-    move: H0 H1.
-    elim a.
-    - move => s f H0 H1.
-    apply inferType_inport_sem_conform.
-    apply H0 with f.
-    apply in_eq.
-    - move => s f H0 H1.
-    apply inferType_outport_sem_conform.
-    apply H1 with f.
-    apply in_eq.
+    elim a; intros; try done.
+    - apply inferType_inport_sem_conform.
+    - apply inferType_outport_sem_conform.
     - rewrite/=.
-    apply H.
-      + move: H0.
-      elim a.
-      intros.
-      simpl.
-      admit.
-      + 
+    apply (H (inferType_port_fun a
+    ce0)). 
+    Qed.
 
   Lemma inferType_inmod_sem_conform :
   forall vm ps ss ce,
     inferType_module (FInmod vm ps ss) ce (inferType_module_fun (FInmod vm ps ss) ce).
   Proof.
     intros.
-    apply infertype_inmod; try done.
+    apply infertype_inmod.
+    simpl.
 
-    rewrite /inferType_module_fun.
+    (*
+    rewrite /CE.add_fst.
 
+    rewrite (CELemmas.add_eq_o _ _ (eq_refl vm)) //.
+    Qed.
+*)
   Admitted.
 
   Lemma inferType_exmod_sem_conform :
@@ -1584,12 +1595,12 @@ Admitted.
 
   Proof.
   Admitted.*)
-
+    
   (** End **)
-
+  
   (********************************************************************************)
 
-
+  
 
   Definition upd_regtyp t r :=
     mk_hfreg t (clock r) (reset r).
@@ -1651,7 +1662,7 @@ Admitted.
     - move => t1 Hm n.
       elim; try done. move => t2 Hn n2.
       move => Heqt; rewrite /= in Heqt.
-      move : Heqt =>/andP[Hteq Heq12].
+      move : Heqt =>/andP[Hteq Heq12]. 
       rewrite (eqP Hteq) /= !eq_refl andTb.
       by apply Hm.
     - move => f1. elim; try discriminate.
@@ -1731,8 +1742,8 @@ Admitted.
          | _, _ => false
          end.
 
-
-
+  
+  
   (* type constraint : dst type ge than src *)
   Definition typeConstraintsGe t1 t2 := typeConstraints geq ltn t1 t2.
 
@@ -1748,7 +1759,7 @@ Admitted.
 
   Fixpoint resolveFlow_fun st te : bool :=
     match st with
-    | Sfcnct r e =>
+    | Sfcnct r e => 
       ftype_equiv (type_of_ref r te) (type_of_hfexpr e te) && valid_rhs_fexpr e te
       && (valid_lhs_orient (orient_of_comp (snd (CE.vtyp (base_ref r) te))))
     | Spcnct r e =>
@@ -1762,7 +1773,7 @@ Admitted.
     | _ => true
     end.
 
-
+  
   (********************************************************************************)
 
   (** Pass InferWidth *)
@@ -1809,7 +1820,7 @@ Admitted.
        | Atyp ta na => CE.add br (upd_vectyp vt t) w
        | Btyp _ => CE.add br (upd_name_ftype vt (v2var (get_field_name rs)) t) w
        end
-     | Esubaccess rs n =>
+     | Esubaccess rs n => 
        let br := base_ref rs in
        let vt := type_of_cmpnttyp (fst (CE.vtyp br ce)) in
        match vt with
@@ -1821,9 +1832,9 @@ Admitted.
        end
      end.
 
-
+   
    (* Require Import FunInd. *)
-
+   
    Fixpoint inferWidth_wmap0 (s : hfstmt) (ce : cenv) (w : wmap0): wmap0 :=
      match s with
      | Snode v e => if is_deftyp (type_of_hfexpr e ce)
@@ -1841,7 +1852,7 @@ Admitted.
        let w2 w := add_ref_wmap0 r2 (type_of_ref r1 ce) ce w in
        if is_deftyp (type_of_ref r1 ce) (*&& (is_deftyp (type_of_ref r2 ce))*) then ((w1 w))
        (*else if ~~ is_deftyp (type_of_ref r1 ce) then w1 w*) else w
-     | Sfcnct r e =>
+     | Sfcnct r e => 
        let w1 := add_ref_wmap0 r (type_of_hfexpr e ce) ce w in
        if is_deftyp (type_of_ref r ce) then w1 else w
      | Spcnct r1 (Eref r2) =>
@@ -1864,7 +1875,7 @@ Admitted.
      (*   if (is_deftyp (type_of_ref rs ce)) *)
      (*   then aux s2 ce (aux s1 ce (w1 w)) *)
      (*   else aux s2 ce (aux s1 ce w) *)
-     | _ => w
+     | _ => w 
      end
    .
 
@@ -1970,17 +1981,17 @@ Admitted.
      forall v,
      new_comp_name v ->
      forall w: wmap0, CE.find v w = None.
-
+     
    Inductive inferWidth_sstmt_sem : hfstmt -> wmap0 -> wmap0 -> cenv -> cenv -> Prop :=
    | inferWidth_sskip wm1 wm2 ce1 ce2 :
-       (forall v t c,
+       (forall v t c, 
        CE.find v ce1 = Some (t, c) ->
        CE.find v wm1 = Some (type_of_cmpnttyp t) ->
        CE.find v wm1 = CE.find v wm2 /\
        CE.find v ce1 = CE.find v ce2) ->
        inferWidth_sstmt_sem (sskip) wm1 wm2 ce1 ce2
    | inferWidth_sstop wm1 wm2 ce1 ce2 ss1 ss2 n :
-       (forall v t c ,
+       (forall v t c , 
        CE.find v ce1 = Some (t, c) ->
        CE.find v wm1 = Some (type_of_cmpnttyp t) ->
        CE.find v wm1 = CE.find v wm2 /\
@@ -1994,7 +2005,7 @@ Admitted.
          CE.find (base_ref v) ce1 = CE.find (base_ref v) ce2) ->
          inferWidth_sstmt_sem (sinvalid v) wm1 wm2 ce1 ce2
    | inferWidth_swhen wm1 wm2 ce1 ce2 c ss1 ss2:
-       (forall v t c ,
+       (forall v t c , 
          CE.find (v) ce1 = Some (t, c) ->
          CE.find (v) wm1 = Some (type_of_cmpnttyp t) ->
          CE.find (v) wm1 = CE.find (v) wm2 /\
@@ -2146,8 +2157,8 @@ Admitted.
      - move => Hwm1.
        move : (CELemmas.add_eq_o wm0 (type_of_hfexpr e ce1) (eq_refl v)) => Hwm01.
        rewrite Hwm01 -Hwm1 -/(wmap_map2_cenv wm1 ce1) -H2.
-       inversion H.
-       move => Ht01.
+       inversion H. 
+       move => Ht01. 
        apply inferWidth_snode_imp; try done.
        rewrite -H5//.
        rewrite Hwm1 (CELemmas.add_eq_o _ _ (eq_refl v))//.
@@ -2233,7 +2244,7 @@ Admitted.
        ce3 = wmap_map2_cenv wm2 ce2 ->
        inferWidth_sstmt_sem (Sreg v r) wm1 wm2 ce2 ce3.
    Proof.
-     intros. rewrite H2.
+     intros. rewrite H2. 
      move : H2.
      move : (new_v_wmap_none H1 wm1) => Hn.
      rewrite/= Hn (negbTE H) => Heqw12.
@@ -2323,9 +2334,9 @@ Admitted.
      rewrite /wmap_map2_cenv.
      have Hnone : (add_width_2_cenv None None = None) by done.
      rewrite (CELemmas.map2_1bis _ _ _ Hnone) (new_v_wmap_none H0 wm1)/=.
-     done.
+     done. 
    Qed.
-
+   
    Lemma sizeof_fgtyp_lt_max_width t1 t2 :
      ftype_equiv (Gtyp t1) (Gtyp t2) ->
      sizeof_fgtyp t1 <= sizeof_fgtyp t2 ->
@@ -2345,19 +2356,19 @@ Admitted.
        elim f ; elim f0; try (intros; rewrite (maxn_idPr H0)//||discriminate||done).
    Admitted.
 
-   Lemma max_width_typeConstraints t1 t2 :
+   Lemma max_width_typeConstraints t1 t2 : 
      ftype_equiv t1 t2 ->
      max_width t1 t2 = t1 ->
      typeConstraintsGe t1 t2.
    Proof. Admitted.
-
+     
    Lemma neg_typeConstraints_max_width t1 t2 :
      ftype_equiv t1 t2 ->
      ~~ (typeConstraintsGe t1 t2) ->
      max_width t1 t2 = t2.
    Proof.
    Admitted.
-
+     
    Lemma ftype_equiv_symmetry t1 t2 :
      ftype_equiv (t1) (t2) -> ftype_equiv (t2) (t1).
    Proof.
@@ -2373,7 +2384,7 @@ Admitted.
      CE.find (base_ref r) wm = Some t1 ->
      CE.find (base_ref r) (add_ref_wmap0 r t2 ce wm) = Some (max_width t1 t2).
    Proof. Admitted.
-
+   
    Lemma inferWidth_sfcnct_ftype_sem_conform :
      forall r e c1 t0 t1 t2 wm1 ce1 wm2 ce2 ,
        ftype_equiv t1 t2 ->
@@ -2412,7 +2423,7 @@ Admitted.
          rewrite Hmw H0/= H2//.
        + move : (neg_typeConstraints_max_width H (negbT Hmax)) => Hmw.
          move : H3 H5.
-         case e; intros;
+         case e; intros; 
          try (apply inferWidth_sfcnct_ftype_gt with (aggr_typ f) t1 (aggr_typ t2) c1;
               [ done
               | rewrite (add_ref_wmap0_max_width _ _ H4) Hmw//
@@ -2446,7 +2457,7 @@ Admitted.
          rewrite Hmw H0/= H2//.
        + move : (neg_typeConstraints_max_width H (negbT Hmax)) => Hmw.
          move : H3 H5.
-         case e; intros;
+         case e; intros; 
            try (apply inferWidth_sfcnct_ftype_gt with (reg_typ h) t1 (reg_typ (mk_freg t2 (clock h) (reset h))) c1;
                 [ done
                 | rewrite (add_ref_wmap0_max_width _ _ H4) Hmw//
@@ -2463,9 +2474,9 @@ Admitted.
      - case Hmax : (typeConstraintsGe t1 t2).
        + move : (typeConstraints_max_width H Hmax) => Hmw.
          move : H3 H5.
-         case e; intros;
+         case e; intros; 
          try (apply inferWidth_sfcnct_ftype_le with
-             (mem_typ h) (mem_typ (mk_fmem t1 (depth h) (reader h) (writer h) (read_latency h) (write_latency h) (read_write h))) t2 c1;
+             (mem_typ h) (mem_typ (mk_fmem t1 (depth h) (reader h) (writer h) (read_latency h) (write_latency h) (read_write h))) t2 c1; 
                 [ done
                 | rewrite -Hmw (add_ref_wmap0_max_width _ _ H4) /=Hmw//
                 | done| done| done
@@ -2480,7 +2491,7 @@ Admitted.
          rewrite (add_ref_wmap0_max_width _ _ H4) H0/= H2 Hmw//.
        + move : (neg_typeConstraints_max_width H (negbT Hmax)) => Hmw.
          move : H3 H5.
-         case e; intros;
+         case e; intros; 
            try (apply inferWidth_sfcnct_ftype_gt with (mem_typ h) t1 (mem_typ (mk_fmem t2 (depth h) (reader h) (writer h) (read_latency h) (write_latency h) (read_write h))) c1;
                 [ done
                 | rewrite (add_ref_wmap0_max_width _ _ H4) Hmw//
@@ -2535,7 +2546,7 @@ Admitted.
          rewrite Hmw H0/= H2//.
        + move : (neg_typeConstraints_max_width H (negbT Hmax)) => Hmw.
          move : H3 H5.
-         case e; intros;
+         case e; intros; 
          try (apply inferWidth_spcnct_ftype_gt with (aggr_typ f) t1 (aggr_typ t2) c1;
               [ done
               | rewrite (add_ref_wmap0_max_width _ _ H4) Hmw//
@@ -2569,7 +2580,7 @@ Admitted.
          rewrite Hmw H0/= H2//.
        + move : (neg_typeConstraints_max_width H (negbT Hmax)) => Hmw.
          move : H3 H5.
-         case e; intros;
+         case e; intros; 
            try (apply inferWidth_spcnct_ftype_gt with (reg_typ h) t1 (reg_typ (mk_freg t2 (clock h) (reset h))) c1;
                 [ done
                 | rewrite (add_ref_wmap0_max_width _ _ H4) Hmw//
@@ -2586,9 +2597,9 @@ Admitted.
      - case Hmax : (typeConstraintsGe t1 t2).
        + move : (typeConstraints_max_width H Hmax) => Hmw.
          move : H3 H5.
-         case e; intros;
+         case e; intros; 
          try (apply inferWidth_spcnct_ftype_le with
-             (mem_typ h) (mem_typ (mk_fmem t1 (depth h) (reader h) (writer h) (read_latency h) (write_latency h) (read_write h))) t2 c1;
+             (mem_typ h) (mem_typ (mk_fmem t1 (depth h) (reader h) (writer h) (read_latency h) (write_latency h) (read_write h))) t2 c1; 
                 [ done
                 | rewrite -Hmw (add_ref_wmap0_max_width _ _ H4) /=Hmw//
                 | done| done| done
@@ -2603,7 +2614,7 @@ Admitted.
          rewrite (add_ref_wmap0_max_width _ _ H4) H0/= H2 Hmw//.
        + move : (neg_typeConstraints_max_width H (negbT Hmax)) => Hmw.
          move : H3 H5.
-         case e; intros;
+         case e; intros; 
            try (apply inferWidth_spcnct_ftype_gt with (mem_typ h) t1 (mem_typ (mk_fmem t2 (depth h) (reader h) (writer h) (read_latency h) (write_latency h) (read_write h))) c1;
                 [ done
                 | rewrite (add_ref_wmap0_max_width _ _ H4) Hmw//
@@ -2620,7 +2631,7 @@ Admitted.
      - rewrite /find_unknown H0 in H7. discriminate.
    Qed.
 
-
+   
    Lemma inferWidth_sfcnct_sem_conform :
      forall v1 e c1 t0 t1 t2 wm1 ce1 wm2 ce2 ,
        ftype_equiv (Gtyp t1) (Gtyp t2) ->
@@ -2652,7 +2663,7 @@ Admitted.
        + rewrite /type_of_hfexpr in H2. rewrite H2.
          apply inferWidth_sfcnct_gtyp_le with c1 t0 t1 t2; try done.
          rewrite Hmw (CELemmas.add_eq_o wm1 (Gtyp t1) (eq_refl v1))//.
-         rewrite H5 H4/wmap_map2_cenv /inferWidth_wmap0 H2.
+         rewrite H5 H4/wmap_map2_cenv /inferWidth_wmap0 H2. 
          rewrite (lock add_ref_wmap0)/= (CE.find_some_vtyp H0) (lock is_deftyp)/= -lock H1/=-lock.
          rewrite /add_ref_wmap0 (lock max_width)/= H3 -lock Hmw.
          rewrite (CELemmas.map2_1bis (CE.add v1 (Gtyp t1) wm1) ce1 v1 Hnone) H0.
@@ -2767,7 +2778,7 @@ Admitted.
      case (is_deftyp (data_type h)); try done.
      case h; intros; rewrite //.
    Qed.
-
+   
    Lemma cefind_eq_eq_width :
      forall v (ce1 ce2 : cenv) t1 t2 c,
        CE.find v ce1 = Some (t1, c) ->
@@ -2776,9 +2787,9 @@ Admitted.
        typeConstraintsGe (type_of_cmpnttyp t2) (type_of_cmpnttyp t1).
    Proof.
    Admitted.
-
+     
    Lemma inferWidth_sstmt_sem_conform :
-     forall st wm1 wm2 ce1 ce2
+     forall st wm1 wm2 ce1 ce2 
        t1 t2,
            (* CE.find (base_ref r) ce1 = Some (t1, c) -> *)
            (* is_deftyp (type_of_cmpnttyp t1) -> *)
@@ -2794,7 +2805,7 @@ Admitted.
    Proof.
    Admitted.
 
-
+   
    Inductive inferWidth_stmts_sem : seq hfstmt -> cenv -> cenv -> Prop :=
    | inferWidth_stmts_nil ce1 ce2 :
        (forall v,
@@ -2818,7 +2829,7 @@ Admitted.
    Proof. Admitted.
 
    Lemma inferType_stmts_hd ss sts ce0 ce1 :
-     inferType_stmts (ss :: sts) ce0 ce1 ->
+     inferType_stmts (ss :: sts) ce0 ce1 -> 
      inferType_stmt ss ce0 ce1.
    Proof.
    Admitted.
@@ -2858,7 +2869,7 @@ Admitted.
            CE.find (base_ref r) ce0 = Some t /\
            is_deftyp (type_of_cmpnttyp (fst t)) /\
            ~~ find_unknown (base_ref r) ce1 /\
-           ~~ is_deftyp (type_of_cmpnttyp (fst (CE.vtyp (base_ref r) (inferWidth_fun sts ce1))))
+           ~~ is_deftyp (type_of_cmpnttyp (fst (CE.vtyp (base_ref r) (inferWidth_fun sts ce1)))) 
            )->
            (* ~~ is_deftyp (type_of_cmpnttyp (fst (CE.vtyp v (inferWidth_fun sts ce1)))) /\ *)
            (*ce2 = wmap_map2_cenv wm1 ce1 /\*)
@@ -2867,19 +2878,19 @@ Admitted.
    Proof.
      have Hnone : (add_width_2_cenv None None = None) by done.
      elim => [ce0 ce1  v He Hiw | st ss Hm ce0 ce1 v He Hiw].
-     -
+     - 
        apply inferWidth_stmts_nil. rewrite /inferWidth_fun/wmap_map2_cenv/=. intro.
-       rewrite (CELemmas.map2_1bis _ _ _ Hnone). rewrite CELemmas.empty_o//.
+       rewrite (CELemmas.map2_1bis _ _ _ Hnone). rewrite CELemmas.empty_o//. 
      -
        case He => [wm0 [wm1 Hec]].
-       apply inferWidth_stmts_imp with (wmap_map2_cenv wm1 ce1).
+       apply inferWidth_stmts_imp with (wmap_map2_cenv wm1 ce1). 
        move : Hec Hiw.
        elim st.
        + (*skip*)
          intros.
          move : (Hec (r) (aggr_typ def_ftype, Node) (* sskip *)) => [Hbrs1 [Hbrt [Hi[Hdt [Hndt [Hun Hit]]]]]].
          (* move : Hbrt => [ [Hinit Hi]].  *) rewrite /= in Hbrt.
-         rewrite //.
+         rewrite //. 
          (* exists wm0; exists wm1. *)
          (* apply inferWidth_sskip_sem_conform; try done. *)
          (* move : (Hec (r) (aggr_typ def_ftype, Node) ) => [Hbrs1 [Hbrt [Hdt [Hndt [Hun Hit]]]]]. *)
@@ -2934,7 +2945,7 @@ Admitted.
          (*            (snd (CE.vtyp (base_ref h) ce1))) => [Hit1 [Hit2 Hit3]]. *)
          (* done. *)
        + (*pcnct*)
-         intros.
+         intros. 
          move : (Hec h (CE.vtyp (base_ref h) ce0) (* (Spcnct h h0) *)) => [Hbrs1 [Hbrt [Hi[Hdt [Hndt [Hun Hit]]]]]].
          rewrite //.
        (* exists wm0; exists wm1. *)
@@ -3028,7 +3039,7 @@ Admitted.
              CE.find (base_ref r) wm0 = Some (type_of_cmpnttyp (fst t)) /\
            is_deftyp (type_of_cmpnttyp (fst t)) /\
            ~~ find_unknown (base_ref r) ce1 /\
-           ~~ is_deftyp (type_of_cmpnttyp (fst (CE.vtyp (base_ref r) (inferWidth_fun sts ce1))))
+           ~~ is_deftyp (type_of_cmpnttyp (fst (CE.vtyp (base_ref r) (inferWidth_fun sts ce1)))) 
            )->
            (* ~~ is_deftyp (type_of_cmpnttyp (fst (CE.vtyp v (inferWidth_fun sts ce1)))) /\ *)
            (*ce2 = wmap_map2_cenv wm1 ce1 /\*)
@@ -3037,12 +3048,12 @@ Admitted.
    Proof.
      have Hnone : (add_width_2_cenv None None = None) by done.
      elim => [ce0 ce1  v He Hiw | st ss Hm ce0 ce1 v He Hiw].
-     -
+     - 
        apply inferWidth_stmts_nil. rewrite /inferWidth_fun/wmap_map2_cenv/=. intro.
-       rewrite (CELemmas.map2_1bis _ _ _ Hnone). rewrite CELemmas.empty_o//.
+       rewrite (CELemmas.map2_1bis _ _ _ Hnone). rewrite CELemmas.empty_o//. 
      -
        case He => [wm0 [wm1 Hec]].
-       apply inferWidth_stmts_imp with (wmap_map2_cenv wm1 ce1).
+       apply inferWidth_stmts_imp with (wmap_map2_cenv wm1 ce1). 
        move : Hec Hiw.
        elim st.
        + (*skip*)
@@ -3055,7 +3066,7 @@ Admitted.
          intros.
          exists wm0; exists wm1.
          move : (Hec (Eid s) (aggr_typ f, Wire) (* (Swire s f) *)) => [Hbrs1 [Hbrt [[Hdt [Hndt [Hun Hit]]]]]].
-         rewrite /= in Hbrt.
+         rewrite /= in Hbrt. 
          move : (new_v_wmap_none Hbrs1 wm0) => Hnv.
          apply inferWidth_swire_sem_conform with ce0; try done.
          exact : (inferType_stmts_hd Hiw).
@@ -3111,10 +3122,10 @@ Admitted.
          rewrite /= in Hdt. rewrite /= in Hbrt; rewrite /= in Hbrs1.
          apply inferWidth_sinvalid; try rewrite //.
    Admitted.
-
+         
    (********************************************************************************)
 
-
+   
    (** Pass InferResets **)
 
    (* A map to store candidate reset signals *)
@@ -3188,7 +3199,7 @@ Admitted.
 
    Definition add_reset2cenv (m : option (list ftype)) (t : option (cmpnt_init_typs * fcomponent)) :=
      match t, m with
-     | Some (Aggr_typ (Gtyp Freset), c), Some rs =>
+     | Some (Aggr_typ (Gtyp Freset), c), Some rs => 
        if (has_async rs && (negb (has_sync rs))) then Some (aggr_typ (Gtyp (Fuint 1)), c)
            else if has_sync rs && has_async rs then Some (aggr_typ def_ftype, c)
                 else Some (aggr_typ (Gtyp (Fuint 1)), c)
@@ -3204,7 +3215,7 @@ Admitted.
 
    (********************************************************************************)
 
-
+   
    (** Pass ExpandConnect *)
 
    Fixpoint size_of_ftype ft :=
@@ -3232,7 +3243,7 @@ Admitted.
      | Btyp b => offset_of_subfield_b b fid n
      end.
 
-   (** TBD *)
+   (** TBD *)  
    Parameter new_var : var -> Var.var -> var.
    Parameter new_subvar : var -> nat -> var.
    Parameter new_subvar_i : var -> nat -> var.
@@ -3240,13 +3251,13 @@ Admitted.
    Parameter var2v : Var.var -> V.t.
    Parameter vtmp : var.
 
-
+      
    Fixpoint list_repeat_fn f n (l : list ftype) :=
      match n with
      | 0 => l
      | S m => list_repeat_fn f m (f l)
      end.
-
+   
    Fixpoint ftype_list (ft : ftype) l :=
      match ft with
      | Gtyp t => Gtyp t :: l
@@ -3259,13 +3270,13 @@ Admitted.
      | Fnil => l
      | Fflips v fl t fs => ftype_list_btyp fs (ftype_list t l)
      end.
-
+   
    Fixpoint vlist_repeat_fn f v i n (l : list (var * ftype)) {struct n}:=
      match n with
      | 0 => l
      | S m => vlist_repeat_fn f (new_subvar v i) i m (f l)
      end.
-
+   
    Fixpoint ftype_vlist v (ft : ftype) l :=
      match ft with
      | Gtyp t => (v, Gtyp t) :: l
@@ -3281,7 +3292,7 @@ Admitted.
 
    (* A map to store types destruct *)
    Definition dmap := CE.t (fgtyp * fcomponent).
-   Definition empty_dmap : dmap := CE.empty (fgtyp * fcomponent).
+   Definition empty_dmap : dmap := CE.empty (fgtyp * fcomponent). 
    Definition findsd (v:var) (d:dmap) :=
      match CE.find v d with Some t => t | None => (Fuint 0, Node)  end.
 
@@ -3292,7 +3303,7 @@ Admitted.
      | Esubindex r n => new_subvar (expand_eref r ce) n
      | Esubaccess r e => new_subvar (expand_eref r ce) 0 (* TBD *)
      end.
-
+   
    (*
    Fixpoint expand_index r t n l : list (var * ftype) :=
      match n with
@@ -3306,7 +3317,7 @@ Admitted.
      | Fflips v fl t fs => expand_fields_fun r fs ((expand_eref (Esubfield r (var2v v)), t) :: l )
      end.
 *)
-
+   
    Fixpoint fcnct_list (l1 :list (var * ftype)) (l2:list (var * ftype)) cs :=
      match l1, l2 with
      | nil, nil => cs
@@ -3329,7 +3340,7 @@ Admitted.
          else pcnct_pair_b v1 v2 t1 fs2 cs
        end
      end.
-
+   
    Fixpoint pcnct_pair (t1 : (var * ftype)) (t2: (var * ftype)) cs :=
      match t1, t2 with
      | (v1, Gtyp t1) , (v2, Gtyp t2) => SV.upd v1 (r_fexpr (Eref (Eid v2))) cs
@@ -3339,9 +3350,9 @@ Admitted.
      | (v1, Btyp b1), (v2, Btyp b2) => pcnct_pair_b v1 v2 b1 b2 cs
      | _, _ => cs
      end.
-
+   
    (* premise : passive type, weak type equiv *)
-
+   
    Parameter store_spcnct : href -> href -> ftype -> cstate -> cstate.
 
    Definition store_rhsexpr (s : hfstmt) (cs : cstate) ce : cstate :=
@@ -3353,16 +3364,16 @@ Admitted.
      | Sfcnct r1 (Eref r2) =>
        let t1 := type_of_ref r1 ce in
        let t2 := type_of_ref r2 ce in
-       fcnct_list (ftype_vlist (expand_eref r1 ce) t1 nil) (ftype_vlist (expand_eref r2 ce) t2 nil) cs
-     | Spcnct r1 (Eref r2) =>
+       fcnct_list (ftype_vlist (expand_eref r1 ce) t1 nil) (ftype_vlist (expand_eref r2 ce) t2 nil) cs 
+     | Spcnct r1 (Eref r2) => 
        let t1 := type_of_ref r1 ce in
        let t2 := type_of_ref r2 ce in
        pcnct_pair (expand_eref r1 ce, t1) (expand_eref r2 ce, t2) cs
      | Sinvalid r1 => SV.upd (expand_eref r1 ce) r_default cs
      | _ => cs
-     end.
+     end.     
 
-
+     
    (*
    (* premise : passive type, type equiv *)
    Fixpoint expand_connect_subindex r1 r2 n : seq hfstmt :=
@@ -3431,7 +3442,7 @@ Admitted.
        expand_fields r1 r2 ffs ce2 cs1 ce' cs' ->
        expand_fields r1 r2 (Fflips (v) f t ffs) ce0 cs0 ce' cs'.
   *)
-
+   
    (*
    Inductive expandConnect : hfstmt -> CE.env -> cstate -> CE.env -> cstate -> Prop :=
    | Expand_fcnnct :
@@ -3452,171 +3463,11 @@ Admitted.
 
    (** Pass ExpandWhens *)
 
-   (* The pass translates a FIRRTL statement sequence (but one without aggregate types/aggregate connects)
-      to one where when statements are replaced by suitable multiplexers or validifs.
-      It also handles the last connect semantics. *)
-
-   Definition map2_helper_cs_tf (c : hfexpr)
-                                (true_expr : option rhs_expr) (false_expr : option rhs_expr) : option rhs_expr :=
-   (* helper function to join connections made in separate branches of a when statement *)
-   match true_expr, false_expr with
-   | None, None (* nowhere declared *)
-   | Some _, None (* declared and defined only in the true branch *)
-   | Some R_default, Some R_default => true_expr (* declared in both branches but nowhere defined *)
-   | None, Some _ => false_expr (* declared and defined only in the false branch *)
-   | Some (R_fexpr t), Some R_default => Some (R_fexpr (Evalidif c t)) (* declared before when, only defined in true branch *)
-   | Some R_default, Some (R_fexpr f) => Some (R_fexpr (Evalidif (Eprim_unop Unot c) f)) (* declared before when, only defined in false branch *)
-   | Some (R_fexpr t), Some (R_fexpr f) => (*if t = f, TBD then true_expr (* both definitions match, no multiplexer needed *)
-                                           else*) Some (R_fexpr (emux c t f)) (* defined differently in both branches *)
-   end.
-
-   Definition combine_branches (c : hfexpr) (true_branch : (seq hfstmt * cstate))
-                                            (false_branch: (seq hfstmt * cstate)) : (seq hfstmt * cstate) :=
-   (* combines the two branches of a when statmeent into one sequence of declaration statements
-      and one map of connections.
-      Input:  * c = condition of the when statement
-              * true_branch = pair of (declaration statements, map of connections),
-                the translation of the true branch of the when statement
-              * false_branch = pair of (declaration statements, map of connections),
-                the translation of the false branch of the when statement
-              Both maps of connections also contain the connections *before* the when statement;
-              this is used if a new connection is only made in one of the branches
-              because the other branch then keeps the value connected to before the when statement.
-      Output: a pair consisting of
-              * declaration statements containing the declarations from both branches
-              * map of connections containing definitions (if necessary using multiplexers/validifs
-                to choose between the values defined in the branches) *)
-         ((fst true_branch) ++ (fst false_branch),
-          SV.map2 (map2_helper_cs_tf c) (snd true_branch) (snd false_branch))
-   .
-
-   Definition stmts_well_order (s1 : seq hfstmt) (s2 : seq hfstmt) : Prop :=
-   (* a well-founded relation to prove that expandBranch_fun is well-founded.
-      (The definition is not transitive but it is sufficient for our purposes.) *)
-   match s2 with
-   | [::] => false
-   | Swhen _ st sf :: ss2 => s1 = st \/ s1 = sf \/ s1 = ss2
-                                       (* The last disjunct can be replaced by:
-                                          stmts_well_order s1 st
-                                       \/ stmts_well_order s1 sf
-                                       \/ stmts_well_order ss1 ss2 *)
-   | _ :: ss2 => s1 = ss2 (* or: _ :: ss1, ... stmts_well_order ss1 ss2 *)
-   end.
-
-   Program Fixpoint expandBranch_fun (ss : seq hfstmt) (ce : cenv) (cs : cstate) { wf stmts_well_order ss } : (seq hfstmt * cstate) :=
-   (* This is the main function of ExpandWhens. It replaces when statements by expressions containing
-      multiplexers/validifs where necessary.  It has the following interface:
-      Input:  * ss = sequence of statements that are a final fragment of a module definition
-                or a final fragment of a branch
-                (not containing partial or aggregate connects;
-                possibly containing double connects and when statements)
-              * ce = component environment, containing the type definitions
-                of the module (this has been found in earlier passes and is not updated)
-              * cs = map of connections that have been defined in the previous statements of the module definition
-                (including, when applicable, in the previous statements of the branch).
-                This map is used in case a when statement only replaces a connect in one branch;
-                in that case, the other branch has to copy the connect from this map.
-      Output: a pair consisting of
-              * sequence of statements, mainly containing declarations of registers and wires,
-                that should become part of the resulting code (because registers and wires etc.
-                declared in one branch should be included always in the translated code)
-              * cstate : map of connects that have been defined before or in the branch
-                (i.e. this map extends parameter cs by the connects in ss). *)
-   match ss with
-   | [::] => ([::], cs)
-   | s :: sss => match s with
-                 | Sinst _ _ (* ignore for now -- TBD *)
-                 | Spcnct _ _ (* should not appear -- ignore *)
-                 | Sskip
-                 | Sinvalid _
-                 | Sstop _ _ _ => expandBranch_fun sss ce cs (* no translation needed *)
-                 | Snode v e => let result := expandBranch_fun sss ce cs (* (SV.upd v (R_fexpr e) cs) *) in
-                                (s :: (fst result), snd result)
-                 | Sreg v r => let result := expandBranch_fun sss ce (SV.upd v (R_fexpr (Eref (Eid v))) cs) in
-                                                                  (* registers keep their old value by default.
-                                                                     The above code works for registers of basic type. *)
-                               (s :: (fst result), snd result)
-                 | Smem v m => let result := expandBranch_fun sss ce cs (* but should assign R_default to all
-                                                                        input signals of ports *) in
-                                (s :: (fst result), snd result)
-                 | Swire v t => let result := expandBranch_fun sss ce (SV.upd v (R_default V.T) cs) in
-                                (s :: (fst result), snd result)
-                 | Sfcnct v e => expandBranch_fun sss ce (SV.upd (expand_eref v ce) (R_fexpr e) cs)
-                 | Swhen c sst ssf => let combined_branches := combine_branches c (expandBranch_fun sst ce cs) (expandBranch_fun ssf ce cs) in
-                                      let result := expandBranch_fun sss ce (snd combined_branches) in
-                                      ((fst combined_branches) ++ (fst result), snd result)
-                 end
-   end.
-   Obligation 1 of expandBranch_fun_func.
-   unfold stmts_well_order ; reflexivity.
-   Qed.
-   Obligation 2 of expandBranch_fun_func.
-   unfold stmts_well_order ; reflexivity.
-   Qed.
-   Obligation 3 of expandBranch_fun_func.
-   unfold stmts_well_order ; reflexivity.
-   Qed.
-   Obligation 4 of expandBranch_fun_func.
-   unfold stmts_well_order ; reflexivity.
-   Qed.
-   Obligation 5 of expandBranch_fun_func.
-   unfold stmts_well_order ; reflexivity.
-   Qed.
-   Obligation 6 of expandBranch_fun_func.
-   unfold stmts_well_order ; reflexivity.
-   Qed.
-   Obligation 7 of expandBranch_fun_func.
-   unfold stmts_well_order ; reflexivity.
-   Qed.
-   Obligation 8 of expandBranch_fun_func.
-   unfold stmts_well_order ; reflexivity.
-   Qed.
-   Obligation 9 of expandBranch_fun_func.
-   unfold stmts_well_order ; reflexivity.
-   Qed.
-   Obligation 10 of expandBranch_fun_func.
-   unfold stmts_well_order ; reflexivity.
-   Qed.
-   Obligation 11 of expandBranch_fun_func.
-   unfold stmts_well_order ; left ; reflexivity.
-   Qed.
-   Obligation 12 of expandBranch_fun_func.
-   unfold stmts_well_order ; right ; left ; reflexivity.
-   Qed.
-   Obligation 13 of expandBranch_fun_func.
-   unfold stmts_well_order ; right ; right ; reflexivity.
-   Qed.
-   Obligation 14 of expandBranch_fun_func.
-   (* Obligation 14 requires to prove that stmts_well_order is actually a well-order.
-      It is because it is based on inductive definition of seq and hfstmt,
-      but I don't know how to write that right now. *)
-   Admitted.
-
-(*
-   Definition expandWhen_fun (ss : seq hfstmt) (ce : cenv) : (seq hfstmt * cstate) := expandBranch_fun ss ce (CE.empty rhs_expr).
-*)
-   (* This function provides an interface to the main function.
-      Input:  * ss = sequence of statements that form a module definition
-                (not containing partial or aggregate connects;
-                possibly containing double connects and when statements)
-              * ce = component environment, containing the type definitions
-                of the module (this has been found in earlier passes and is not updated)
-      Output: same as the main function expandBranch_fun.
-
-      The output can be used to generate a lowered FIRRTL module definition,
-      where the statements would be the statement sequence of the output,
-      extended by connects for all elements of the output map.
-      However, for the verification of correctness, it is easier to directly
-      verify the map instead of the generated code. *)
-
-   (* Definition expandWhen1_fun s ce cs : seq hfstmt := *)
+   (* Definition expandWhens_fun s ce cs : hfstmt := *)
    (*   match s with *)
-   (*   | Swhen c ss1 ss2 => (* first collect all connections and nodes from ss1 and ss2; if some overlap, create a multiplexer;
-                                                                                if there is no overlap create a multiplexer with the previous value or a validif.
-                                Copy register / wire / memory definitions as they appear in the branches. *) *)
-   (*   | _ => s :: [::] *)
+   (*   | Swhen c (Sfcnct r e) s2 =>  *)
 
-   (* Fixpoint expandWhens_stmts_sem ... -- DNJ will think about this. *)
+
 
   (** Semantics of declaim  ports*)
   Inductive eval_port : hfport -> CE.env -> cstate -> CE.env -> cstate -> Prop :=
@@ -3735,7 +3586,7 @@ Admitted.
     | Some R_default, Some (R_fexpr e_t) => Some (R_fexpr e_t)
     | Some er1, None => Some er1
     | None, Some er2 => Some er2
-    | _, _ => None
+    | _, _ => None 
     end.
 
   Definition merge_branch_cs_e c re re_e : option rhs_expr :=
@@ -3745,7 +3596,7 @@ Admitted.
     | Some R_default, Some (R_fexpr e_e) => Some (R_fexpr e_e)
     | Some er1, None => Some er1
     | None, Some er2 => Some er2
-    | _, _ => None
+    | _, _ => None 
     end.
 
   Definition merge_branch_ce ce ce_t : option (cmpnt_init_typs * fcomponent) :=
@@ -3755,7 +3606,7 @@ Admitted.
     | Some (Reg_typ t1, cp1), Some (Aggr_typ t2, cp2) => Some (Reg_typ t1, cp1)
     | Some er1, None => Some er1
     | None, Some er2 => Some er2
-    | _, _ => None
+    | _, _ => None 
     end.
 
 
@@ -3850,13 +3701,13 @@ Admitted.
   (* Lemma valid_conncection v e2 sts ce cs ce' cs' : *)
   (*   eval_fstmts_group (sfcnct (eref v) e2 :: sts) ce cs ce' cs' -> *)
   (*   valid_rhs (SV.acc v cs') ce'. *)
-
-
+    
+       
    (********************************************************************************)
-
+            
 
    (** Pass LowerTypes *)
-   (* lower ports
+   (* lower ports 
     * We lower ports in a separate pass in order to ensure that statements inside the module do not influence port names.*)
     (* Dependency(RemoveAccesses), // we require all SubAccess nodes to have been removed *)
     (* Dependency(CheckTypes), // we require all types to be correct *)
@@ -3898,14 +3749,14 @@ Admitted.
        | 0 => l
        | S n => destructTypes_fun_aux (new_var r (N.of_nat n)) t c l
        end
-     | Btyp bs => destructField_fun_aux r bs c l
+     | Btyp bs => destructField_fun_aux r bs c l 
      end
      with destructField_fun_aux r bs c l :=
             match bs with
             | Fnil => l
             | Fflips v f t ff =>
               match f with
-              | Nflip =>
+              | Nflip => 
                 destructTypes_fun_aux (new_var r v) t c l ++ destructField_fun_aux r ff c l
               | Flipped =>
                 destructTypes_fun_aux (new_var r v) t (io_conv c) l ++ destructField_fun_aux r ff c l
@@ -3947,7 +3798,7 @@ Admitted.
    Definition lowerTypes_fun ss ce : CE.env :=
      dmap_2_cenv (lowerTypes_init_fstmts ss empty_dmap) ce.
 
-
+   
    (********************************************************************************)
 
    (** Pass RemoveReset *)
@@ -3956,19 +3807,19 @@ Admitted.
      match rt with | Gtyp Fasyncreset => true | _ => false end.
 
    Parameter invalid_value : ftype.
-
+   
    Definition RemoveReset_fun (st : hfstmt) ce ss :=
      match st with
      | Sreg v r => match (reset r) with
-                   | Rst er (Eref (Eid ei)) =>
+                   | Rst er (Eref (Eid ei)) => 
                      match (SV.acc ei ss) with
                      | R_default =>
-                       (CE.add_fst v
+                       (CE.add_fst v 
                                    (Reg_typ (mk_freg (type r) (clock r) (Rst (econst (Fuint 1) [::b0]) (eref (eid v))))) ce, ss)
                      | _ => (ce, ss)
                      end
                    | Rst (Econst t [::b0]) ei =>
-                     (CE.add_fst v
+                     (CE.add_fst v 
                             (Reg_typ (mk_freg (type r) (clock r) (Rst (econst (Fuint 1) [::b0]) (eref (eid v))))) ce, ss)
                    | Rst e1 ei => if is_async e1 ce then (ce, ss)
                                   else (CE.add_fst v (Reg_typ (mk_freg (type r) (clock r) (Rst (econst (Fuint 1) [::b0]) (eref (eid v))))) ce, ss)
@@ -4003,8 +3854,8 @@ Admitted.
        end
      | _ => (ce, ss)
      end.
-
-
+   
+  
 End MakeHiFirrtl.
 
 
